New apply implementation with full correctness proof

Bdd/Apply.lean
@@ -4,123 +4,1528 @@ import Std.Data.HashMap.Lemmas
 
 namespace Apply
 
-abbrev p2t : Nat → Nat → Nat := fun l r ↦ (l + 2) * (r + 2)
+private def RawPointer := Bool ⊕ Nat
 
-private structure State (n) (m) (m') where
-  cache : Std.HashMap (Pointer m × Pointer m') (Pointer (p2t m m'))
-  heap : Vector (Node n (p2t m m')) (p2t m m')
-  next : Fin (p2t m m')
+private structure RawNode (n) where
+  va : Fin n
+  lo : RawPointer
+  hi : RawPointer
 
-private def GoodState (op : Bool → Bool → Bool) (Ov : Vector (Node n m) m) (Uv : Vector (Node n m') m') : State n m m' → Prop := fun s ↦
-  ∀ key (hk : key ∈ s.cache),
-  ∃ (o : Bdd.Ordered ⟨s.heap, s.cache[key]'hk⟩) (o1 : Bdd.Ordered ⟨Ov, key.1⟩) (o2 : Bdd.Ordered ⟨Uv, key.2⟩),
-  ∀ I,
-  (op (OBdd.evaluate ⟨⟨Ov, key.1⟩, o1⟩ I) (OBdd.evaluate ⟨⟨Uv, key.2⟩, o2⟩ I)) = OBdd.evaluate ⟨⟨s.heap, s.cache[key]'hk⟩, o⟩ I
+private def RawPointer.Bounded (m : Nat) (p : RawPointer) := ∀ {i}, p = .inr i → i < m
 
--- def threeval (op : (Bool → Bool → Bool)) : Pointer m → Pointer m' → (Option Bool)
---   | .terminal b => fun
---     | .terminal b' => op b b'
---     | .node _ => if (op b false) = (op b true) then some (op b false) else none
---   | .node _ => fun
---     | .terminal b' => if (op false b') = (op true b') then some (op false b') else none
---     | .node _ => none
+private def RawPointer.bounded_of_le {p : RawPointer} (hm : p.Bounded m) (h : m ≤ m') : p.Bounded m' := by
+  intro i hi
+  cases hp : p with
+  | inl val => simp_all
+  | inr val =>
+    have := hm hp
+    simp_all
+    injection hi with heq
+    subst heq
+    omega
 
--- def apply_helper (nid : Fin (m * m')) (heap : Vector (Node n (m * m')) (m * m')) (cache : Std.HashMap (Pointer m × Pointer m') (Pointer (m * m'))) (op : (Bool → Bool → Bool)) (O : OBdd n m) (U : OBdd n' m') :
---     Bdd n (m * m') :=
---   match cache.get? ⟨O.1.root, U.1.root⟩ with
---   | some root => ⟨heap, root⟩
---   | none =>
---     if (threeval op O.1.root U.1.root) = none
---     then
---       sorry
---     else sorry
+private def RawPointer.cook (p : RawPointer) (h : p.Bounded m) : Pointer m :=
+  match p with
+  | .inl b => .terminal b
+  | .inr i => .node ⟨i, h rfl⟩
 
--- def apply_helper {n m m' : Nat} (op : (Bool → Bool → Bool)) (O : OBdd n m.succ) (U : OBdd n' m'.succ) :
---     StateM (State n m.succ m'.succ) (Pointer (m.succ * m'.succ)) := do
---   let s ← get
---   match s.cache.get? ⟨O.1.root, U.1.root⟩ with
---   | some root => pure root
---   | none =>
---     match threeval op O.1.root U.1.root with
---     | some b =>
---       set (⟨s.cache.insert ⟨O.1.root, U.1.root⟩ (.terminal b), s.heap, s.next⟩ : State n m.succ m'.succ)
---       pure (.terminal b)
---     | none =>
---       if O.var ≤ U.var
---       then
---         if O.var ≥ U.var
---         then
--- --        set (⟨s.cache.insert ⟨O.1.root, U.1.root⟩ (.node s.next), s.heap.set s.next sorry, s.next + 1⟩ : State n m.succ m'.succ)
---           pure (.node s.next)
---         else sorry
---       else sorry
+private lemma RawPointer.cook_equiv {h1 : Apply.RawPointer.Bounded m1 p} {h2 : Apply.RawPointer.Bounded m2 p} : Pointer.equiv (RawPointer.cook p h1) (RawPointer.cook p h2) := by
+  simp only [Pointer.equiv]
+  constructor
+  · intro b hb
+    cases p <;> simp_all [RawPointer.cook]
+  · intro j hj
+    cases p with
+    | inl val => contradiction
+    | inr val =>
+      simp only [Bounded] at h1 h2
+      simp only [cook, Pointer.node.injEq] at hj
+      rw [Fin.eq_mk_iff_val_eq] at hj
+      simp only at hj
+      subst hj
+      use ⟨j.1, h2 rfl⟩
+      simp [RawPointer.cook]
 
-private def cache_get {n m m' : Nat} (O_root : Pointer m) (U_root : Pointer m') :
-    StateM (State n m m') (Option (Pointer (p2t m m'))) := fun s ↦
-  ⟨(s.cache.get? ⟨O_root, U_root⟩), s⟩
+private def RawPointer.fromPointer : Pointer m → RawPointer
+  | .terminal b => .inl b
+  | .node j => .inr j.1
 
-private lemma mem_cache_of_cache_get_eq_some : (cache_get l r s).1.isSome → ⟨l, r⟩ ∈ s.cache := by
-  simp only [cache_get]
+private def RawNode.Bounded (m : Nat) (N : RawNode n) := N.lo.Bounded m ∧ N.hi.Bounded m
+
+private def RawNode.bounded_of_le {N : RawNode n} (hm : N.Bounded m) (h : m ≤ m') : N.Bounded m' :=
+  ⟨RawPointer.bounded_of_le hm.1 h, RawPointer.bounded_of_le hm.2 h⟩
+
+private def RawNode.cook (N : RawNode n) (h : N.Bounded m) : Node n m := ⟨N.va, N.lo.cook h.1, N.hi.cook h.2⟩
+
+private lemma RawNode.cook_equiv : Node.equiv (RawNode.cook N h1) (RawNode.cook N h2) := by
+  simp only [Node.equiv]
+  constructor
+  · rfl
+  · rcases h1 with ⟨h11, h12⟩
+    rcases h2 with ⟨h21, h22⟩
+    constructor
+    · apply RawPointer.cook_equiv <;> assumption
+    · apply RawPointer.cook_equiv <;> assumption
+
+private def cook_heap {n c} (heap : Vector (RawNode n) c) (hh : ∀ i : Fin c, RawNode.Bounded i heap[i]) : Vector (Node n c) c :=
+  Vector.ofFn (fun i ↦ heap[i].cook (RawNode.bounded_of_le (hh i) (by omega)))
+
+private structure State (n) (n') (m) (m') where
+  size : Nat
+  heap : Vector (RawNode (max n n')) size
+  cache : Std.HashMap (Pointer m × Pointer m') RawPointer
+
+private def initial : State n n' m m' := ⟨_, (Vector.emptyWithCapacity 0), Std.HashMap.emptyWithCapacity⟩
+
+def toVar_or (M : Vector (Node n m) m) : Pointer m → Nat → Nat
+  | .terminal _, i => i
+  | .node j, _     => M[j].var
+
+@[simp]
+lemma toVar_or_terminal_eq {n m} (w : Vector (Node n m) m) : toVar_or w (.terminal b) i = i := rfl
+
+@[simp]
+lemma toVar_or_node_eq {n m} (w : Vector (Node n m) m) {j} : toVar_or w (.node j) i = w[j].var := rfl
+
+private def Invariant (op : Bool → Bool → Bool) (O : OBdd n m) (U : OBdd n' m') (r : State n n' m m') :=
+  ∃ hh : (∀ i : Fin r.size, RawNode.Bounded i r.heap[i]),
+    ∀ (k : (Pointer m × Pointer m')) (p : RawPointer),
+      r.cache[k]? = some p →
+      (∀ j h, p = .inr j → (r.heap[j]'h).va.1 =
+        (toVar_or O.1.heap k.1 (n ⊔ n')) ⊓ (toVar_or U.1.heap k.2 (n ⊔ n'))) ∧
+      ∃ hk1 : Bdd.Ordered ⟨O.1.heap, k.1⟩,
+        ∃ hk2 : Bdd.Ordered ⟨U.1.heap, k.2⟩,
+          ∃ hp : p.Bounded r.size,
+            ∃ o : Bdd.Ordered ⟨cook_heap r.heap hh, p.cook hp⟩,
+              ∀ I,
+                OBdd.evaluate ⟨⟨cook_heap r.heap hh, p.cook hp⟩, o⟩ I =
+                op
+                  (OBdd.evaluate ⟨⟨O.1.heap, k.1⟩, hk1⟩ (Vector.cast (by simp) (I.take n)))
+                  (OBdd.evaluate ⟨⟨U.1.heap, k.2⟩, hk2⟩ (Vector.cast (by simp) (I.take n')))
+
+private lemma inv_initial {op} {O : OBdd n m} {U : OBdd n' m'} : Invariant op O U initial := by
+  constructor
+  · intro k p hp
+    simp only [initial, Std.HashMap.getElem?_emptyWithCapacity, reduceCtorEq] at hp
+  · rintro ⟨_, c⟩
+    simp only [initial, not_lt_zero'] at c
+
+private def cache_get (O_root : Pointer m) (U_root : Pointer m') (s : (State n n' m m')) : (Option RawPointer) :=
+  s.cache[(⟨O_root, U_root⟩ : (Pointer m × Pointer m'))]?
+
+private lemma cook_low {rn : RawNode n} {h1} {h2} : rn.lo.cook (m := m) h1 = (rn.cook h2).low := rfl
+
+private lemma cook_high {rn : RawNode n} {h1} {h2} : rn.hi.cook (m := m) h1 = (rn.cook h2).high := rfl
+
+private lemma cook_inj {p q : RawPointer} {hp} {hq} : p.cook (m := m) hp = q.cook hq → p = q := by
   intro h
-  simp_all only [Std.HashMap.get?_eq_getElem?, isSome_getElem?]
+  cases p <;> cases q <;> simp_all [RawPointer.cook]
 
-private lemma cache_get_preserves_state : (cache_get l r s).2 = s := by
-  simp only [cache_get]
+private lemma cook_aux {p : RawPointer} {h1} {h2} : p.cook h1 = .node j → p.cook h2 = .node ⟨j, hj⟩ := by
+  intro h
+  cases p with
+  | inl val => simp_all [RawPointer.cook]
+  | inr val =>
+    simp_all [RawPointer.cook]
+    rw [Fin.eq_mk_iff_val_eq] at h
+    exact h
 
-private def cache_put {n m m' : Nat} (O_root : Pointer m) (U_root : Pointer m') (val : Pointer (p2t m m')) :
-    StateM (State n m m') Unit := fun s ↦
-  ⟨(), ⟨s.cache.insert ⟨O_root, U_root⟩ val, s.heap, s.next⟩⟩
+private lemma push_ordered_aux {v : Vector (RawNode n) m} {h0} {h2} : Pointer.Reachable (cook_heap (v.push N) h2) (RawPointer.cook p h3) q → ∀ j, q = .node j → ∃ hj : j.1 < m, Pointer.Reachable (cook_heap v h0) (p.cook h1) (.node ⟨j.1, hj⟩) := by
+  intro h
+  induction h with
+  | refl =>
+    intro i hi
+    cases p with
+    | inl val => contradiction
+    | inr val =>
+      simp [RawPointer.cook] at hi
+      subst hi
+      simp only
+      use h1 rfl
+      simp [RawPointer.cook]
+      left
+  | tail r e ih =>
+    intro j hj
+    rename_i b c
+    cases e with
+    | low heq =>
+      rename_i jb
+      have := h2 jb
+      simp only [RawNode.Bounded] at this
+      simp only [cook_heap, Fin.getElem_fin, Vector.getElem_ofFn] at heq
+      subst hj
+      have that : (v.push N)[jb].lo = .inr j.1 := by
+        rw [show Pointer.node j = RawPointer.cook (.inr j.1) _ by rfl] at heq
+        rw [← cook_low] at heq
+        exact cook_inj heq
+        apply RawPointer.bounded_of_le this.1
+        omega
+        simp [RawPointer.Bounded]
+        intro i hi
+        injection hi with heq
+        rw [← heq]
+        omega
+      have : Apply.RawPointer.Bounded (↑jb) (v.push N)[jb].lo := this.1
+      have := this that
+      use lt_of_lt_of_le this (Nat.le_of_lt_succ jb.2)
+      rcases (ih jb rfl) with ⟨r1, r2⟩
+      trans .node ⟨jb.1, r1⟩
+      · exact r2
+      · simp_rw [Vector.getElem_push_lt r1] at heq
+        right
+        left
+        left
+        simp [cook_heap, RawNode.cook]
+        simp [cook_heap, RawNode.cook] at heq
+        exact cook_aux heq
+    | high heq =>
+      rename_i jb
+      have := h2 jb
+      simp only [RawNode.Bounded] at this
+      simp only [cook_heap, Fin.getElem_fin, Vector.getElem_ofFn] at heq
+      subst hj
+      have that : (v.push N)[jb].hi = .inr j.1 := by
+        rw [show Pointer.node j = RawPointer.cook (.inr j.1) _ by rfl] at heq
+        rw [← cook_high] at heq
+        exact cook_inj heq
+        apply RawPointer.bounded_of_le this.2
+        omega
+        simp [RawPointer.Bounded]
+        intro i hi
+        injection hi with heq
+        rw [← heq]
+        omega
+      have : Apply.RawPointer.Bounded (↑jb) (v.push N)[jb].hi := this.2
+      have := this that
+      use lt_of_lt_of_le this (Nat.le_of_lt_succ jb.2)
+      rcases (ih jb rfl) with ⟨r1, r2⟩
+      trans .node ⟨jb.1, r1⟩
+      · exact r2
+      · simp_rw [Vector.getElem_push_lt r1] at heq
+        right
+        left
+        right
+        simp [cook_heap, RawNode.cook]
+        simp [cook_heap, RawNode.cook] at heq
+        exact cook_aux heq
 
--- TODO: also call cache_put in heap_push
--- def heap_push {n m m' : Nat} (N : Node n (p2t m m')) :
---     StateM (State n m m') Unit := fun s ↦
---   ⟨(), ⟨s.cache, s.heap.set s.next N, s.next + 1⟩⟩
+private lemma push_ordered : Bdd.Ordered ⟨cook_heap v h0, RawPointer.cook p h1⟩ → Bdd.Ordered ⟨cook_heap (v.push N) h2, RawPointer.cook p h3⟩ := by
+  intro h
+  apply Bdd.ordered_of_ordered_heap_all_reachable_eq ⟨⟨cook_heap v h0, RawPointer.cook p h1⟩, h⟩
+  · intro j hj
+    rcases (push_ordered_aux hj (h2 := h2) (h1 := h1) (h0 := h0) j rfl) with ⟨r1, r2⟩
+    use r1
+    simp only [cook_heap, Fin.getElem_fin, Vector.getElem_ofFn, Vector.getElem_push_lt r1,
+      RawNode.cook_equiv]
+  · intro j hj
+    simp_all only
+    simp [RawPointer.cook] at hj
+    split at hj
+    next heq => contradiction
+    next heq =>
+      simp only [Pointer.node.injEq] at hj
+      subst hj
+      use h1 rfl
+      simp [RawPointer.cook]
 
-private def heap_push {n m m' : Nat} (O_root : Pointer m) (U_root : Pointer m') (N : Node n (p2t m m')) :
-    StateM (State n m m') (Pointer (p2t m m')) := fun s ↦
-  ⟨.node s.next, ⟨s.cache.insert ⟨O_root, U_root⟩ (.node s.next), s.heap.set s.next N, s.next + 1⟩⟩
+private lemma push_evaluate {v : Vector _ _} {h0} {h1} {ho : Bdd.Ordered _} {hu : Bdd.Ordered ⟨cook_heap v h1, RawPointer.cook p hq⟩} :
+    OBdd.evaluate ⟨⟨cook_heap (v.push N) h0, RawPointer.cook p hp⟩, ho⟩ =
+    OBdd.evaluate ⟨⟨cook_heap v h1, RawPointer.cook p hq⟩, hu⟩ := by
+  apply OBdd.evaluate_eq_evaluate_of_ordered_heap_all_reachable_eq
+  · simp only [Fin.getElem_fin]
+    intro j hj
+    use (by omega)
+    simp only [cook_heap, Fin.getElem_fin, Vector.getElem_ofFn, Fin.is_lt, Vector.getElem_push_lt]
+    exact RawNode.cook_equiv
+  · exact RawPointer.cook_equiv (h2 := hp)
 
-private def next : StateM (State n m m') (Fin (p2t m m')) := fun s ↦ ⟨s.next, s⟩
+private lemma heap_push_aux (s : (State n n' m m')) (inv : Invariant op O U s)
+    (hNl : ∃ k : Pointer m × Pointer m', s.cache[k]? = some N.lo)
+    (hNh : ∃ k : Pointer m × Pointer m', s.cache[k]? = some N.hi)
+    (hNv : N.va.1 = (toVar_or O.1.heap O.1.root (n ⊔ n')) ⊓ (toVar_or U.1.heap U.1.root (n ⊔ n')))
+    (hxl : ∀ j h (_ : N.lo = .inr j), N.va.1 < (s.heap[j]'h).va.1)
+    (hxh : ∀ j h (_ : N.hi = .inr j), N.va.1 < (s.heap[j]'h).va.1)
+    (hh : ∀ h0 (h1 : Bdd.Ordered _) (I : Vector Bool (max n n')),
+            OBdd.evaluate ⟨{ heap := Apply.cook_heap (s.heap.push N) h0, root := Pointer.node ⟨s.size, by simp⟩ }, h1⟩ I =
+            op (O.evaluate (Vector.cast (by omega) (I.extract 0 n))) (U.evaluate (Vector.cast (by omega) (I.extract 0 n')))) :
+    Invariant op O U
+      { size := s.size + 1, heap := s.heap.push N, cache := s.cache.insert (O.1.root, U.1.root) (Sum.inr s.size) } := by
+  rcases hNl with ⟨kl, hkl⟩
+  rcases hNh with ⟨kh, hkh⟩
+  have hN : RawNode.Bounded s.size N := by
+    simp only [RawNode.Bounded]
+    constructor
+    · exact (inv.2 kl N.lo hkl).2.2.2.1
+    · exact (inv.2 kh N.hi hkh).2.2.2.1
+  have : ∀ (i : Fin (s.size + 1)), Apply.RawNode.Bounded (↑i) (s.heap.push N)[i] := by
+    intro i
+    simp only [Fin.getElem_fin]
+    rw [Vector.getElem_push]
+    split
+    next hi => exact inv.1 ⟨i.1, hi⟩
+    next hi =>
+      have : i.1 = s.size := by omega
+      rw [this]
+      exact hN
+  use this
+  intro k p
+  simp only
+  intro hp
+  rw [Std.HashMap.getElem?_insert] at hp
+  simp only [beq_iff_eq, Vector.take_eq_extract] at hp
+  split at hp
+  next heq =>
+    subst heq
+    simp only
+    constructor
+    · intro j hs hj
+      rw [Vector.getElem_push]
+      split
+      next heqq =>
+        injection hp with hpp
+        rw [hj] at hpp
+        injection hpp with hppp
+        rw [hppp] at heqq
+        absurd heqq
+        simp only [lt_self_iff_false, not_false_eq_true]
+      next heqq =>
+        exact hNv
+    use O.2, U.2
+    injection hp with hpe
+    subst hpe
+    have hb : Apply.RawPointer.Bounded (s.size + 1) (Sum.inr s.size) := by intro i hi; injection hi with hie; subst hie; simp
+    use hb
+    have hoo : Bdd.Ordered ⟨Apply.cook_heap (s.heap.push N) this, Apply.RawPointer.cook (Sum.inr s.size) hb⟩ := by
+      apply Bdd.ordered_of_low_high_ordered rfl
+      · simp only [Bdd.low, cook_heap]
+        simp only [Fin.getElem_fin, Vector.getElem_ofFn, Vector.getElem_push_eq]
+        rw [← cook_low]
+        swap; apply RawPointer.bounded_of_le (inv.2 kl N.lo hkl).2.2.2.1; simp only [le_add_iff_nonneg_right, zero_le]
+        rcases (inv.2 kl N.lo hkl).2.2.2 with that
+        apply push_ordered
+        · exact this
+        · exact that.2.1
+      ·
+        simp [Nat.succ_eq_add_one, Bdd.var, gt_iff_lt, cook_heap, Bdd.low, RawPointer.cook]
+        cases heq : N.lo with
+        | inl val =>
+          rw [← cook_low]
+          simp_rw [heq]
+          simp only [RawPointer.cook, Pointer.toVar_terminal_eq, Nat.succ_eq_add_one,
+            Fin.natCast_eq_last, Fin.castSucc_lt_last]
+          apply RawPointer.bounded_of_le (inv.2 kl N.lo hkl).2.2.2.1; simp only [le_add_iff_nonneg_right, zero_le]
+        | inr val =>
+          have hvs : val < s.size := by
+            apply RawPointer.bounded_of_le (inv.2 kl N.lo hkl).2.2.2.1 .refl heq
+          rw [← cook_low]
+          simp_rw [heq]
+          simp only [RawNode.cook, RawPointer.cook, Pointer.toVar_node_eq, Nat.succ_eq_add_one,
+            Fin.getElem_fin, Vector.getElem_ofFn, Fin.coe_eq_castSucc, Fin.castSucc_lt_castSucc_iff]
+          rw [Vector.getElem_push_lt]
+          have hvs : val < s.size := by
+            apply RawPointer.bounded_of_le (inv.2 kl N.lo hkl).2.2.2.1 .refl heq
+          exact hxl _ hvs heq
+          exact hvs
+          apply RawPointer.bounded_of_le (inv.2 kl N.lo hkl).2.2.2.1; simp only [le_add_iff_nonneg_right, zero_le]
+      · simp only [Bdd.high, cook_heap]
+        simp only [Fin.getElem_fin, Vector.getElem_ofFn, Vector.getElem_push_eq]
+        rw [← cook_high]
+        swap; apply RawPointer.bounded_of_le (inv.2 kh N.hi hkh).2.2.2.1; simp only [le_add_iff_nonneg_right, zero_le]
+        rcases (inv.2 kh N.hi hkh).2.2.2 with that
+        apply push_ordered
+        · exact this
+        · exact that.2.1
+      ·
+        simp [Nat.succ_eq_add_one, Bdd.var, gt_iff_lt, cook_heap, Bdd.high, RawPointer.cook]
+        cases heq : N.hi with
+        | inl val =>
+          rw [← cook_high]
+          simp_rw [heq]
+          simp only [RawPointer.cook, Pointer.toVar_terminal_eq, Nat.succ_eq_add_one,
+            Fin.natCast_eq_last, Fin.castSucc_lt_last]
+          apply RawPointer.bounded_of_le (inv.2 kh N.hi hkh).2.2.2.1; simp only [le_add_iff_nonneg_right, zero_le]
+        | inr val =>
+          have hvs : val < s.size := by
+            apply RawPointer.bounded_of_le (inv.2 _ _ hkh).2.2.2.1 .refl heq
+          rw [← cook_high]
+          simp_rw [heq]
+          simp only [RawNode.cook, RawPointer.cook, Pointer.toVar_node_eq, Nat.succ_eq_add_one,
+            Fin.getElem_fin, Vector.getElem_ofFn, Fin.coe_eq_castSucc, Fin.castSucc_lt_castSucc_iff]
+          rw [Vector.getElem_push_lt]
+          exact hxh _ hvs heq
+          apply RawPointer.bounded_of_le (inv.2 kh N.hi hkh).2.2.2.1; simp only [le_add_iff_nonneg_right, zero_le]
+    use hoo
+    rw [show ⟨{ heap := U.1.heap, root := U.1.root }, _⟩ =  U by rfl]
+    rw [show ⟨{ heap := O.1.heap, root := O.1.root }, _⟩ =  O by rfl]
+    simp only [RawPointer.cook]
+    intro I
+    apply hh _ hoo
+  next heq =>
+    constructor
+    · intro j hs hj
+      rw [hj] at hp
+      rcases (inv.2 k _ hp) with ⟨inv1, inv2⟩
+      have := inv1 j (inv2.2.2.1 rfl) rfl
+      rw [Vector.getElem_push_lt (inv2.2.2.1 rfl)]
+      exact this
+    rcases (inv.2 k p hp) with that
+    use that.2.1
+    use that.2.2.1
+    have hb : ∀ {i}, p = Sum.inr i → i < s.size + 1 :=
+      RawPointer.bounded_of_le that.2.2.2.1 (by simp only [le_add_iff_nonneg_right, zero_le])
+    use hb
+    have ho : Bdd.Ordered { heap := Apply.cook_heap (s.heap.push N) this, root := p.cook hb } := push_ordered that.2.2.2.2.1
+    use ho
+    intro I
+    calc _
+      _ = OBdd.evaluate ⟨{ heap := Apply.cook_heap (s.heap) inv.1, root := p.cook that.2.2.2.1 }, that.2.2.2.2.1⟩ I := by
+        rw [OBdd.evaluate_eq_evaluate_of_ordered_heap_all_reachable_eq]
+        · simp only [Fin.getElem_fin]
+          intro j hj
+          use (by omega)
+          simp [cook_heap]
+          exact RawNode.cook_equiv
+        · simp only [RawPointer.cook_equiv]
+    exact that.2.2.2.2.2 I
 
-private def apply_helper {n m m' : Nat} (op : (Bool → Bool → Bool)) (O : OBdd n m) (U : OBdd n m') :
-    StateM (State n m m') (Pointer (p2t m m')) := do
-  let cache_hit ← cache_get O.1.root U.1.root
-  match cache_hit with
-  | some root => pure root
+private def heap_push (N : RawNode (n ⊔ n')) (s : (State n n' m m')) (inv : Invariant op O U s)
+    (hNl : ∃ k : Pointer m × Pointer m', s.cache[k]? = some N.lo)
+    (hNh : ∃ k : Pointer m × Pointer m', s.cache[k]? = some N.hi)
+    (hNv : N.va.1 = (toVar_or O.1.heap O.1.root (n ⊔ n')) ⊓ (toVar_or U.1.heap U.1.root (n ⊔ n')))
+    (hxl : ∀ j h (_ : N.lo = .inr j), N.va.1 < (s.heap[j]'h).va.1)
+    (hxh : ∀ j h (_ : N.hi = .inr j), N.va.1 < (s.heap[j]'h).va.1)
+    (hh : ∀ h0 (h1 : Bdd.Ordered _) (I : Vector Bool (max n n')),
+            OBdd.evaluate ⟨{ heap := Apply.cook_heap (s.heap.push N) h0, root := Pointer.node ⟨s.size, by simp⟩ }, h1⟩ I =
+            op (O.evaluate (Vector.cast (by omega) (I.extract 0 n))) (U.evaluate (Vector.cast (by omega) (I.extract 0 n'))))
+            (hc : s.cache[(⟨O.1.root, U.1.root⟩ : Pointer m × Pointer m')]? = none ) :
+    { r : State n n' m m' × RawPointer //
+      (Invariant op O U r.1) ∧
+      (r.1.cache[(⟨O.1.root, U.1.root⟩ : Pointer m × Pointer m')]? = some r.2) ∧
+      s.size ≤ r.1.size ∧
+      (∀ (k : Pointer m × Pointer m'),
+        (∀ p, s.cache[k]? = some p → r.1.cache[k]? = some p) ∧
+        (r.1.cache[k]? = none → s.cache[k]? = none) ∧
+        (s.cache[k]? = none → (∃ p, r.1.cache[k]? = some p) → Pointer.Reachable O.1.heap O.1.root k.1 ∧ Pointer.Reachable U.1.heap U.1.root k.2)) ∧
+      (∀ j h, r.2 = .inr j → (r.1.heap[j]'h).va.1 = (toVar_or O.1.heap O.1.root (n ⊔ n')) ⊓ (toVar_or U.1.heap U.1.root (n ⊔ n')))
+    } :=
+  ⟨⟨⟨s.size + 1, s.heap.push N, s.cache.insert ⟨O.1.root, U.1.root⟩ (.inr s.size)⟩, .inr s.size⟩, by
+    simp only [Prod.exists]
+    constructor
+    · exact heap_push_aux s inv hNl hNh hNv hxl hxh hh
+    · constructor
+      · simp only [Std.HashMap.getElem?_insert_self]
+      · constructor
+        · simp only [le_add_iff_nonneg_right, zero_le]
+        · constructor
+          swap
+          · intro j hj1 hj2
+            injection hj2 with hji
+            subst hji
+            simp only [Vector.getElem_push_eq]
+            exact hNv
+          intro k
+          constructor
+          · intro p hkp
+            rw [← hkp]
+            simp only [Std.HashMap.getElem?_insert, beq_iff_eq, ite_eq_right_iff]
+            intro contra
+            rw [← contra] at hkp
+            rw [hkp] at hc
+            contradiction
+          · constructor
+            · simp only [getElem?_eq_none_iff, Std.HashMap.mem_insert, beq_iff_eq, not_or,
+                and_imp, imp_self, implies_true]
+            · rintro hk ⟨q, hq⟩
+              simp only [Std.HashMap.getElem?_insert, beq_iff_eq, ite_eq_right_iff] at hq
+              split at hq
+              next heqq => subst heqq; constructor <;> left
+              next heqq => rw [hk] at hq; contradiction
+  ⟩
+
+private lemma insert_terminal_invariant (s0 : State n n' m m') (inv : Invariant op O U s0) (ho : O.1.root = .terminal b) (hu : U.1.root = .terminal b'):
+    Invariant op O U { size := s0.size, heap := s0.heap, cache := s0.cache.insert (O.1.root, U.1.root) (Sum.inl (op b b')) } := by
+  constructor
+  intro k p hp
+  simp only at hp
+  simp only
+  rw [Std.HashMap.getElem?_insert] at hp
+  simp only [beq_iff_eq] at hp
+  split at hp
+  next heq =>
+    rw [← heq]
+    constructor
+    · intro j hj hjp
+      subst hjp
+      injection hp with hpp
+      contradiction
+    use O.2, U.2
+    injection hp with hpe
+    subst hpe
+    use (fun contra ↦ by contradiction)
+    simp [RawPointer.cook, ho, hu, Bdd.Ordered_of_terminal]
+  next =>
+    constructor
+    · exact (inv.2 _ _ hp).1
+    exact (inv.2 _ _ hp).2
+
+private lemma op_if1 (op : Bool → Bool → Bool) {c l rt rf : Bool} :
+    op l (if c then rt else rf) = if c then (op l rt) else (op l rf) :=
+      apply_ite (op l) (c = true) rt rf
+
+private lemma op_if2 (op : Bool → Bool → Bool) {c lt lf r : Bool} :
+    op  (if c then lt else lf) r = if c then (op lt r) else (op lf r) := by
+  split
+  next h =>
+    subst h
+    simp_all only
+  next h => simp_all only [Bool.not_eq_true]
+
+private lemma op_if3 (op : Bool → Bool → Bool) {c lt lf rt rf : Bool} :
+    op (if c then lt else lf) (if c then rt else rf) = if c then (op lt rt) else (op lf rf) := by
+  split
+  next h =>
+    subst h
+    simp_all only
+  next h => simp_all only [Bool.not_eq_true]
+
+private lemma aux_lt1_low {O : OBdd n m} {U : OBdd n' m'} (O_root_def : O.1.root = .terminal b) (U_root_def : U.1.root = .node j') :
+    U.1.heap[j'].var.1 <
+    min (toVar_or O.1.heap O.1.root (max n n'))
+        (toVar_or U.1.heap (U.low U_root_def).1.root (max n n')) := by
+  have := OBdd.var_lt_low_var (h := U_root_def)
+  simp_all [OBdd.var, toVar_or, Pointer.toVar]
+  split <;> simp_all
+
+private lemma aux_lt1_high {O : OBdd n m} {U : OBdd n' m'} (O_root_def : O.1.root = .terminal b) (U_root_def : U.1.root = .node j') :
+    U.1.heap[j'].var.1 <
+    min (toVar_or O.1.heap O.1.root (max n n'))
+        (toVar_or U.1.heap (U.high U_root_def).1.root (max n n')) := by
+  have := OBdd.var_lt_low_var (h := U_root_def)
+  have := OBdd.var_lt_high_var (h := U_root_def)
+  simp_all [OBdd.var, toVar_or, Pointer.toVar]
+  split <;> simp_all
+
+private lemma aux_lt2_low {O : OBdd n m} {U : OBdd n' m'} (O_root_def : O.1.root = .node j) (U_root_def : U.1.root = .terminal b') :
+    O.1.heap[j].var.1 <
+    min (toVar_or O.1.heap (O.low O_root_def).1.root (max n n'))
+        (toVar_or U.1.heap U.1.root (max n n')) := by
+  have := OBdd.var_lt_low_var (h := O_root_def)
+  have := OBdd.var_lt_high_var (h := O_root_def)
+  simp_all [OBdd.var, toVar_or, Pointer.toVar]
+  split <;> simp_all
+
+private lemma aux_lt2_high {O : OBdd n m} {U : OBdd n' m'} (O_root_def : O.1.root = .node j) (U_root_def : U.1.root = .terminal b') :
+    O.1.heap[j].var.1 <
+    min (toVar_or O.1.heap (O.high O_root_def).1.root (max n n'))
+        (toVar_or U.1.heap U.1.root (max n n')) := by
+  have := OBdd.var_lt_low_var (h := O_root_def)
+  have := OBdd.var_lt_high_var (h := O_root_def)
+  simp_all [OBdd.var, toVar_or, Pointer.toVar]
+  split <;> simp_all
+
+private lemma aux_lt3_low {O : OBdd n m} {U : OBdd n' m'} (O_root_def : O.1.root = .node j) (U_root_def : U.1.root = .node j') (hleq : O.1.heap[j].var.1 < U.1.heap[j'].var.1) :
+    O.1.heap[j].var.1 <
+    min (toVar_or O.1.heap (O.low O_root_def).1.root (max n n'))
+        (toVar_or U.1.heap U.1.root (max n n')) := by
+  have := OBdd.var_lt_low_var (h := O_root_def)
+  have := OBdd.var_lt_high_var (h := O_root_def)
+  have := OBdd.var_lt_low_var (h := U_root_def)
+  have := OBdd.var_lt_high_var (h := U_root_def)
+  simp_all [OBdd.var, toVar_or, Pointer.toVar]
+  split <;> simp_all
+
+private lemma aux_lt3_high {O : OBdd n m} {U : OBdd n' m'} (O_root_def : O.1.root = .node j) (U_root_def : U.1.root = .node j') (hleq : O.1.heap[j].var.1 < U.1.heap[j'].var.1) :
+    O.1.heap[j].var.1 <
+    min (toVar_or O.1.heap (O.high O_root_def).1.root (max n n'))
+        (toVar_or U.1.heap U.1.root (max n n')) := by
+  have := OBdd.var_lt_low_var (h := O_root_def)
+  have := OBdd.var_lt_high_var (h := O_root_def)
+  have := OBdd.var_lt_low_var (h := U_root_def)
+  have := OBdd.var_lt_high_var (h := U_root_def)
+  simp_all [OBdd.var, toVar_or, Pointer.toVar]
+  split <;> simp_all
+
+private lemma aux_lt4_low {O : OBdd n m} {U : OBdd n' m'} (O_root_def : O.1.root = .node j) (U_root_def : U.1.root = .node j') (hgeq : O.1.heap[j].var.1 > U.1.heap[j'].var.1) :
+    U.1.heap[j'].var.1 <
+    min (toVar_or O.1.heap O.1.root (max n n'))
+        (toVar_or U.1.heap (U.low U_root_def).1.root (max n n')) := by
+  have := OBdd.var_lt_low_var (h := O_root_def)
+  have := OBdd.var_lt_high_var (h := O_root_def)
+  have := OBdd.var_lt_low_var (h := U_root_def)
+  have := OBdd.var_lt_high_var (h := U_root_def)
+  simp_all [OBdd.var, toVar_or, Pointer.toVar]
+  split <;> simp_all
+
+private lemma aux_lt4_high {O : OBdd n m} {U : OBdd n' m'} (O_root_def : O.1.root = .node j) (U_root_def : U.1.root = .node j') (hgeq : O.1.heap[j].var.1 > U.1.heap[j'].var.1) :
+    U.1.heap[j'].var.1 <
+    min (toVar_or O.1.heap O.1.root (max n n'))
+        (toVar_or U.1.heap (U.high U_root_def).1.root (max n n')) := by
+  have := OBdd.var_lt_low_var (h := O_root_def)
+  have := OBdd.var_lt_high_var (h := O_root_def)
+  have := OBdd.var_lt_low_var (h := U_root_def)
+  have := OBdd.var_lt_high_var (h := U_root_def)
+  simp_all [OBdd.var, toVar_or, Pointer.toVar]
+  split <;> simp_all
+
+private lemma aux_lt5_low {O : OBdd n m} {U : OBdd n' m'} (O_root_def : O.1.root = .node j) (U_root_def : U.1.root = .node j') (heeq : O.1.heap[j].var.1 = U.1.heap[j'].var.1) :
+    U.1.heap[j'].var.1 <
+    min (toVar_or O.1.heap (O.low O_root_def).1.root (max n n'))
+        (toVar_or U.1.heap (U.low U_root_def).1.root (max n n')) := by
+  have h1 := OBdd.var_lt_low_var (h := O_root_def)
+  have h2 := OBdd.var_lt_high_var (h := O_root_def)
+  have h3 := OBdd.var_lt_low_var (h := U_root_def)
+  have h4 := OBdd.var_lt_high_var (h := U_root_def)
+  have h5 : U.1.heap[↑j'].var.1 < n + 1 := by omega
+  simp_all [OBdd.var, toVar_or, heeq]
+  split
+  next heq =>
+    split
+    next heqq => simp_all
+    next heqq => simp_all
+  next heq =>
+    split
+    next heqq =>
+      have h6 : (U.1.heap[↑j'].var.1) % (n + 1) = U.1.heap[↑j'].var.1 := by exact Nat.mod_eq_of_lt h5
+      simp_all only [Fin.getElem_fin]
+      simp_all
+    next heqq =>
+      have h6 : (U.1.heap[↑j'].var.1) % (n + 1) = U.1.heap[↑j'].var.1 := by exact Nat.mod_eq_of_lt h5
+      simp_all only [Fin.getElem_fin]
+      simp_all
+
+private lemma aux_lt5_high {O : OBdd n m} {U : OBdd n' m'} (O_root_def : O.1.root = .node j) (U_root_def : U.1.root = .node j') (heeq : O.1.heap[j].var.1 = U.1.heap[j'].var.1) :
+    U.1.heap[j'].var.1 <
+    min (toVar_or O.1.heap (O.high O_root_def).1.root (max n n'))
+        (toVar_or U.1.heap (U.high U_root_def).1.root (max n n')) := by
+  have h2 := OBdd.var_lt_high_var (h := O_root_def)
+  have h3 := OBdd.var_lt_low_var (h := U_root_def)
+  have h4 := OBdd.var_lt_high_var (h := U_root_def)
+  have h5 : U.1.heap[↑j'].var.1 < n + 1 := by omega
+  simp_all [OBdd.var, toVar_or, heeq]
+  split
+  next heq =>
+    split
+    next heqq => simp_all
+    next heqq => simp_all
+  next heq =>
+    split
+    next heqq =>
+      have h6 : (U.1.heap[↑j'].var.1) % (n + 1) = U.1.heap[↑j'].var.1 := by exact Nat.mod_eq_of_lt h5
+      simp_all only [Fin.getElem_fin]
+      simp_all
+    next heqq =>
+      have h6 : (U.1.heap[↑j'].var.1) % (n + 1) = U.1.heap[↑j'].var.1 := by exact Nat.mod_eq_of_lt h5
+      simp_all only [Fin.getElem_fin]
+      simp_all
+
+private def apply_helper (op : (Bool → Bool → Bool)) (O : OBdd n m) (U : OBdd n' m') (s0 : State n n' m m') (inv : Invariant op O U s0) :
+    { r : State n n' m m' × RawPointer //
+      (Invariant op O U r.1) ∧
+      (r.1.cache[(⟨O.1.root, U.1.root⟩ : Pointer m × Pointer m')]? = some r.2) ∧
+      (s0.size ≤ r.1.size) ∧
+      (∀ (k : Pointer m × Pointer m'),
+        (∀ p, s0.cache[k]? = some p → r.1.cache[k]? = some p) ∧
+        (r.1.cache[k]? = none → s0.cache[k]? = none) ∧
+        (s0.cache[k]? = none → (∃ p, r.1.cache[k]? = some p) → Pointer.Reachable O.1.heap O.1.root k.1 ∧ Pointer.Reachable U.1.heap U.1.root k.2)) ∧
+      (∀ j h, r.2 = .inr j → (r.1.heap[j]'h).va.1 = (toVar_or O.1.heap O.1.root (n ⊔ n')) ⊓ (toVar_or U.1.heap U.1.root (n ⊔ n')))
+    } :=
+  match hc : cache_get O.1.root U.1.root s0 with
+  | some root =>
+    ⟨ ⟨s0, root⟩, ⟨inv, hc, .refl,
+      by
+        intro k
+        constructor
+        · intro p h
+          exact h
+        · constructor
+          · intro h
+            exact h
+          · rintro h ⟨_, c⟩
+            rw [h] at c
+            contradiction,
+      by
+        simp only [Nat.succ_eq_add_one, Bdd.var]
+        intro j hj1 hj2
+        simp only [cache_get] at hc
+        rw [hj2] at hc
+        exact (inv.2 _ _ hc).1 _ _ rfl
+      ⟩
+    ⟩
   | none =>
     match O_root_def : O.1.root with
     | .terminal b =>
       match U_root_def : U.1.root with
       | .terminal b' =>
-        let b'' := op b b'
-        cache_put O.1.root U.1.root (.terminal b'')
-        pure (.terminal b'')
+        ⟨⟨⟨s0.size, s0.heap, s0.cache.insert ⟨O.1.root, U.1.root⟩ (.inl (op b b'))⟩, .inl (op b b')⟩, by
+          simp only [Prod.exists]
+          constructor
+          · exact insert_terminal_invariant s0 inv O_root_def U_root_def
+          · constructor
+            · simp only [O_root_def, U_root_def, Std.HashMap.getElem?_insert_self]
+            · constructor
+              · exact .refl
+              · constructor
+                intro k
+                constructor
+                · intro p hp
+                  simp only [cache_get] at hc
+                  rw [← hp]
+                  simp only [Std.HashMap.getElem?_insert, beq_iff_eq, ite_eq_right_iff]
+                  intro contra
+                  subst contra
+                  rw [hc] at hp
+                  contradiction
+                · constructor
+                  · simp only [getElem?_eq_none_iff, Std.HashMap.mem_insert, beq_iff_eq, not_or,
+                      and_imp, imp_self, implies_true]
+                  · rintro h1 ⟨p, hp⟩
+                    simp only [Std.HashMap.getElem?_insert,beq_iff_eq] at hp
+                    split at hp
+                    next heq =>
+                      subst heq
+                      simp only [O_root_def, U_root_def]
+                      constructor
+                      · left
+                      · left
+                    next heq => rw [h1] at hp; contradiction
+                · intro _ _ _; contradiction
+        ⟩
       | .node j' =>
-        let l ← apply_helper op O (U.low  U_root_def)
-        let h ← apply_helper op O (U.high U_root_def)
-        heap_push O.1.root U.1.root ⟨U.1.heap[j'].var, l, h⟩
+        let ⟨⟨sl, rl⟩, ⟨invl, hl, hsl, hlp⟩⟩ := apply_helper op O (U.low U_root_def) s0 inv
+        let ⟨⟨sh, rh⟩, ⟨invh, hh, hsh, hhp⟩⟩ := apply_helper op O (U.high U_root_def) sl invl
+        let ⟨r, ⟨invv, hv, hsv, hvp⟩⟩ :=
+          heap_push (O := O) (U := U)
+            ⟨⟨U.1.heap[j'].var.1, by omega⟩, rl, rh⟩ sh invh
+            (by
+              use ⟨O.1.root, ((U.low U_root_def).1.root)⟩
+              simp only
+              exact (hhp.1 _).1 _ hl
+            )
+            ⟨_, hh⟩
+            (by
+              simp only
+              rw [O_root_def, U_root_def]
+              simp only [Fin.getElem_fin, toVar_or, le_sup_iff, Fin.is_le', or_true,
+                inf_of_le_right]
+            )
+            (by
+              intro j hj1
+              simp only [Fin.getElem_fin]
+              intro hj2
+              have := (hhp.1 _).1 _ hl
+              simp only at this
+              rw [hj2] at this
+              have that := (invh.2 _ (.inr j) this).1 _ hj1 rfl
+              simp only at that
+              rw [that]
+              exact aux_lt1_low O_root_def U_root_def
+            )
+            (by
+              intro j hj1
+              simp only [Fin.getElem_fin]
+              intro hj2
+              have := hhp.2 _ hj1 hj2
+              rw [this]
+              exact aux_lt1_high O_root_def U_root_def
+            )
+            (by
+              intro h0 h1 I
+              symm
+              rw [OBdd.evaluate_node'' U_root_def]
+              simp only
+              rw [op_if1 op]
+              simp only [OBdd.evaluate_node]
+              congr 1
+              · simp only [Nat.sub_zero, Fin.getElem_fin, Vector.getElem_cast, cook_heap,
+                  RawNode.cook, Vector.getElem_ofFn, Vector.getElem_push_eq, eq_iff_iff,
+                  Bool.coe_iff_coe]
+                have := Vector.getElem_extract (as := I) (start := 0) (stop := n') (i := U.1.heap[j'.1].var.1) (by omega)
+                simp only [Nat.sub_zero, zero_add] at this
+                exact this
+              · conv =>
+                  rhs
+                  congr
+                  congr
+                  congr
+                  rfl
+                  simp [cook_heap, RawNode.cook]
+                  rfl
+                  rfl
+                symm
+                have := (invh.2 ⟨O.1.root, (U.high U_root_def).1.root⟩ rh hh).2
+                calc _
+                  _ = OBdd.evaluate ⟨⟨cook_heap sh.heap _, rh.cook _⟩, _⟩ I := by
+                    rw [push_evaluate]
+                    · exact this.2.2.1
+                    · exact push_ordered this.2.2.2.1
+                    · exact this.2.2.2.1
+                  _ = _ := by
+                    have := this.2.2.2.2 I
+                    simp only [Vector.take_eq_extract, OBdd.high_heap_eq_heap] at this
+                    exact this
+              · conv =>
+                  rhs
+                  congr
+                  congr
+                  congr
+                  rfl
+                  simp [cook_heap, RawNode.cook]
+                  rfl
+                  rfl
+                symm
+                have : sh.cache[(⟨O.1.root, (U.low U_root_def).1.root⟩ : Pointer m × Pointer m')]? = some rl := by
+                  apply (hhp.1 _).1
+                  exact hl
+                have := invh.2 ⟨O.1.root, (U.low U_root_def).1.root⟩ rl this
+                calc _
+                  _ = OBdd.evaluate ⟨⟨cook_heap sh.heap _, rl.cook _⟩, _⟩ I := by
+                    rw [push_evaluate]
+                    · exact this.2.2.2.1
+                    · exact push_ordered this.2.2.2.2.1
+                    · exact this.2.2.2.2.1
+                  _ = _ := by
+                    have := this.2.2.2.2.2 I
+                    simp only [Vector.take_eq_extract, OBdd.high_heap_eq_heap] at this
+                    exact this
+            )
+            (by
+              simp only [cache_get] at hc
+              cases heq : sh.cache[(⟨O.1.root, U.1.root⟩ : Pointer m × Pointer m')]? with
+              | none => rfl
+              | some val =>
+                cases heqq : sl.cache[(⟨O.1.root, U.1.root⟩ : Pointer m × Pointer m')]? with
+                | none =>
+                  have := ((hhp.1 _).2.2 heqq ⟨val, heq⟩).2
+                  simp only [OBdd.high_heap_eq_heap] at this
+                  absurd this
+                  apply OBdd.not_oedge_reachable
+                  exact oedge_of_high
+                | some val =>
+                  have := ((hlp.1 _).2.2 hc ⟨_, heqq⟩).2
+                  simp only [OBdd.low_heap_eq_heap] at this
+                  absurd this
+                  apply OBdd.not_oedge_reachable
+                  exact oedge_of_low
+            )
+        ⟨ r,
+          invv,
+          (by rw [O_root_def, U_root_def] at hv; exact hv),
+          .trans hsl (.trans hsh hsv),
+          by
+            constructor
+            swap
+            · rw [← O_root_def, ← U_root_def]
+              exact hvp.2
+            intro k
+            constructor
+            · intro p hp
+              apply (hvp.1 _).1
+              apply (hhp.1 _).1
+              apply (hlp.1 _).1
+              exact hp
+            · constructor
+              · intro hk
+                apply (hlp.1 _).2.1
+                apply (hhp.1 _).2.1
+                apply (hvp.1 _).2.1
+                exact hk
+              · intro hk hkp
+                rw [← O_root_def, ← U_root_def]
+                cases heq : sh.cache[k]? with
+                | none =>
+                  apply (hvp.1 _).2.2 heq hkp
+                | some w =>
+                  cases heqq : sl.cache[k]? with
+                  | none =>
+                    have := (hhp.1 _).2.2 heqq ⟨_, heq⟩
+                    constructor
+                    · exact this.1
+                    · trans (U.high U_root_def).1.root
+                      · apply OBdd.reachable_of_edge
+                        exact oedge_of_high.2
+                      · exact this.2
+                  | some ww =>
+                    have := (hlp.1 _).2.2 hk ⟨_, heqq⟩
+                    constructor
+                    · exact this.1
+                    · trans (U.low U_root_def).1.root
+                      · apply OBdd.reachable_of_edge
+                        exact oedge_of_low.2
+                      · exact this.2
+        ⟩
     | .node j =>
       match U_root_def : U.1.root with
       | .terminal b' =>
-        let l ← apply_helper op (O.low  O_root_def) U
-        let h ← apply_helper op (O.high O_root_def) U
-        heap_push O.1.root U.1.root ⟨O.1.heap[j].var, l, h⟩
+        let ⟨⟨sl, rl⟩, ⟨invl, hl, hsl, hlp⟩⟩ := apply_helper op (O.low O_root_def) U s0 inv
+        let ⟨⟨sh, rh⟩, ⟨invh, hh, hsh, hhp⟩⟩ := apply_helper op (O.high O_root_def) U sl invl
+        let ⟨r, ⟨invv, hv, hsv, hvp⟩⟩ :=
+          heap_push (O := O) (U := U)
+            ⟨⟨O.1.heap[j].var.1, by omega⟩, rl, rh⟩ sh invh
+            ⟨_, (hhp.1 _).1 _ hl⟩
+            ⟨_, hh⟩
+            (by
+              simp only
+              rw [O_root_def, U_root_def]
+              simp only [Fin.getElem_fin, toVar_or, le_sup_iff, Fin.is_le', or_true, true_or,
+                inf_of_le_right, inf_of_le_left]
+            )
+            (by
+              intro j hj1
+              simp only [Fin.getElem_fin]
+              intro hj2
+              have := (hhp.1 _).1 _ hl
+              simp only at this
+              rw [hj2] at this
+              have that := (invh.2 _ (.inr j) this).1 _ hj1 rfl
+              simp only at that
+              rw [that]
+              exact aux_lt2_low O_root_def U_root_def
+            )
+            (by
+              intro j hj1
+              simp only [Fin.getElem_fin]
+              intro hj2
+              have := hhp.2 _ hj1 hj2
+              rw [this]
+              exact aux_lt2_high O_root_def U_root_def
+            )
+            (by
+              intro h0 h1 I
+              symm
+              rw [OBdd.evaluate_node'' O_root_def]
+              simp only
+              rw [op_if2 op]
+              simp only [OBdd.evaluate_node]
+              congr 1
+              · simp only [Nat.sub_zero, Fin.getElem_fin, Vector.getElem_cast, cook_heap,
+                  RawNode.cook, Vector.getElem_ofFn, Vector.getElem_push_eq, eq_iff_iff,
+                  Bool.coe_iff_coe]
+                have := Vector.getElem_extract (as := I) (start := 0) (stop := n) (i := O.1.heap[j.1].var.1) (by omega)
+                simp only [Nat.sub_zero, zero_add] at this
+                exact this
+              · conv =>
+                  rhs
+                  congr
+                  congr
+                  congr
+                  rfl
+                  simp [cook_heap, RawNode.cook]
+                  rfl
+                  rfl
+                symm
+                have := (invh.2 ⟨(O.high O_root_def).1.root, U.1.root⟩ rh hh).2
+                calc _
+                  _ = OBdd.evaluate ⟨⟨cook_heap sh.heap _, rh.cook _⟩, _⟩ I := by
+                    rw [push_evaluate]
+                    · exact this.2.2.1
+                    · exact push_ordered this.2.2.2.1
+                    · exact this.2.2.2.1
+                  _ = _ := by
+                    have := this.2.2.2.2 I
+                    simp only [Vector.take_eq_extract, OBdd.high_heap_eq_heap] at this
+                    exact this
+              · conv =>
+                  rhs
+                  congr
+                  congr
+                  congr
+                  rfl
+                  simp [cook_heap, RawNode.cook]
+                  rfl
+                  rfl
+                symm
+                have : sh.cache[(⟨(O.low O_root_def).1.root, U.1.root⟩ : Pointer m × Pointer m')]? = some rl := by
+                  apply (hhp.1 _).1
+                  exact hl
+                have := invh.2 ⟨(O.low O_root_def).1.root, U.1.root⟩ rl this
+                calc _
+                  _ = OBdd.evaluate ⟨⟨cook_heap sh.heap _, rl.cook _⟩, _⟩ I := by
+                    rw [push_evaluate]
+                    · exact this.2.2.2.1
+                    · exact push_ordered this.2.2.2.2.1
+                    · exact this.2.2.2.2.1
+                  _ = _ := by
+                    have := this.2.2.2.2.2 I
+                    simp only [Vector.take_eq_extract, OBdd.high_heap_eq_heap] at this
+                    exact this
+            )
+            (by
+              simp only [cache_get] at hc
+              cases heq : sh.cache[(⟨O.1.root, U.1.root⟩ : Pointer m × Pointer m')]? with
+              | none => rfl
+              | some val =>
+                cases heqq : sl.cache[(⟨O.1.root, U.1.root⟩ : Pointer m × Pointer m')]? with
+                | none =>
+                  have := ((hhp.1 _).2.2 heqq ⟨val, heq⟩).1
+                  simp only [OBdd.high_heap_eq_heap] at this
+                  absurd this
+                  apply OBdd.not_oedge_reachable
+                  exact oedge_of_high
+                | some val =>
+                  have := ((hlp.1 _).2.2 hc ⟨_, heqq⟩).1
+                  simp only [OBdd.low_heap_eq_heap] at this
+                  absurd this
+                  apply OBdd.not_oedge_reachable
+                  exact oedge_of_low
+            )
+        ⟨ r,
+          invv,
+          (by rw [O_root_def, U_root_def] at hv; exact hv),
+          .trans hsl (.trans hsh hsv),
+          by
+            constructor
+            swap
+            · rw [← O_root_def, ← U_root_def]
+              exact hvp.2
+            intro k
+            constructor
+            · intro p hp
+              apply (hvp.1 _).1
+              apply (hhp.1 _).1
+              apply (hlp.1 _).1
+              exact hp
+            · constructor
+              · intro hk
+                apply (hlp.1 _).2.1
+                apply (hhp.1 _).2.1
+                apply (hvp.1 _).2.1
+                exact hk
+              · intro hk hkp
+                rw [← O_root_def, ← U_root_def]
+                cases heq : sh.cache[k]? with
+                | none =>
+                  apply (hvp.1 _).2.2 heq hkp
+                | some w =>
+                  cases heqq : sl.cache[k]? with
+                  | none =>
+                    have := (hhp.1 _).2.2 heqq ⟨_, heq⟩
+                    constructor
+                    · trans (O.high O_root_def).1.root
+                      · apply OBdd.reachable_of_edge
+                        exact oedge_of_high.2
+                      · exact this.1
+                    · exact this.2
+                  | some ww =>
+                    have := (hlp.1 _).2.2 hk ⟨_, heqq⟩
+                    constructor
+                    · trans (O.low O_root_def).1.root
+                      · apply OBdd.reachable_of_edge
+                        exact oedge_of_low.2
+                      · exact this.1
+                    · exact this.2
+        ⟩
       | .node j' =>
-        if O.1.heap[j].var < U.1.heap[j'].var
+        if hleq : O.1.heap[j].var.1 < U.1.heap[j'].var.1
         then
-          let l ← apply_helper op (O.low  O_root_def) U
-          let h ← apply_helper op (O.high O_root_def) U
-          heap_push O.1.root U.1.root ⟨O.1.heap[j].var, l, h⟩
+          let ⟨⟨sl, rl⟩, ⟨invl, hl, hsl, hlp⟩⟩ := apply_helper op (O.low O_root_def) U s0 inv
+          let ⟨⟨sh, rh⟩, ⟨invh, hh, hsh, hhp⟩⟩ := apply_helper op (O.high O_root_def) U sl invl
+          let ⟨r, ⟨invv, hv, hsv, hvp⟩⟩ :=
+            heap_push (O := O) (U := U)
+              ⟨⟨O.1.heap[j].var.1, by omega⟩, rl, rh⟩ sh invh
+              ⟨_, (hhp.1 _).1 _ hl⟩
+              ⟨_, hh⟩
+              (by
+                simp only
+                rw [O_root_def, U_root_def]
+                simp only [Fin.getElem_fin, toVar_or, le_sup_iff, Fin.is_le', or_true, true_or,
+                  inf_of_le_right, inf_of_le_left]
+                exact Eq.symm (min_eq_left_of_lt hleq)
+              )
+              (by
+                intro j'' hj1
+                simp only [Fin.getElem_fin]
+                intro hj2
+                have := (hhp.1 _).1 _ hl
+                simp only at this
+                rw [hj2] at this
+                have that := (invh.2 _ _ this).1 _ hj1 rfl
+                simp only at that
+                rw [that]
+                exact aux_lt3_low O_root_def U_root_def hleq
+              )
+              (by
+                intro j'' hj1
+                simp only [Fin.getElem_fin]
+                intro hj2
+                have := hhp.2 _ hj1 hj2
+                rw [this]
+                exact aux_lt3_high O_root_def U_root_def hleq
+              )
+              (by
+                intro h0 h1 I
+                symm
+                rw [OBdd.evaluate_node'' O_root_def]
+                simp only
+                rw [op_if2 op]
+                simp only [OBdd.evaluate_node]
+                congr 1
+                · simp only [Nat.sub_zero, Fin.getElem_fin, Vector.getElem_cast, cook_heap,
+                    RawNode.cook, Vector.getElem_ofFn, Vector.getElem_push_eq, eq_iff_iff,
+                    Bool.coe_iff_coe]
+                  have := Vector.getElem_extract (as := I) (start := 0) (stop := n) (i := O.1.heap[j.1].var.1) (by omega)
+                  simp only [Nat.sub_zero, zero_add] at this
+                  exact this
+                · conv =>
+                    rhs
+                    congr
+                    congr
+                    congr
+                    rfl
+                    simp [cook_heap, RawNode.cook]
+                    rfl
+                    rfl
+                  symm
+                  have := (invh.2 ⟨(O.high O_root_def).1.root, U.1.root⟩ rh hh).2
+                  calc _
+                    _ = OBdd.evaluate ⟨⟨cook_heap sh.heap _, rh.cook _⟩, _⟩ I := by
+                      rw [push_evaluate]
+                      · exact this.2.2.1
+                      · exact push_ordered this.2.2.2.1
+                      · exact this.2.2.2.1
+                    _ = _ := by
+                      have := this.2.2.2.2 I
+                      simp only [Vector.take_eq_extract, OBdd.high_heap_eq_heap] at this
+                      exact this
+                · conv =>
+                    rhs
+                    congr
+                    congr
+                    congr
+                    rfl
+                    simp [cook_heap, RawNode.cook]
+                    rfl
+                    rfl
+                  symm
+                  have : sh.cache[(⟨(O.low O_root_def).1.root, U.1.root⟩ : Pointer m × Pointer m')]? = some rl := by
+                    apply (hhp.1 _).1
+                    exact hl
+                  have := invh.2 ⟨(O.low O_root_def).1.root, U.1.root⟩ rl this
+                  calc _
+                    _ = OBdd.evaluate ⟨⟨cook_heap sh.heap _, rl.cook _⟩, _⟩ I := by
+                      rw [push_evaluate]
+                      · exact this.2.2.2.1
+                      · exact push_ordered this.2.2.2.2.1
+                      · exact this.2.2.2.2.1
+                    _ = _ := by
+                      have := this.2.2.2.2.2 I
+                      simp only [Vector.take_eq_extract, OBdd.high_heap_eq_heap] at this
+                      exact this
+              )
+              (by
+                simp only [cache_get] at hc
+                cases heq : sh.cache[(⟨O.1.root, U.1.root⟩ : Pointer m × Pointer m')]? with
+                | none => rfl
+                | some val =>
+                  cases heqq : sl.cache[(⟨O.1.root, U.1.root⟩ : Pointer m × Pointer m')]? with
+                  | none =>
+                    have := ((hhp.1 _).2.2 heqq ⟨val, heq⟩).1
+                    simp only [OBdd.high_heap_eq_heap] at this
+                    absurd this
+                    apply OBdd.not_oedge_reachable
+                    exact oedge_of_high
+                  | some val =>
+                    have := ((hlp.1 _).2.2 hc ⟨_, heqq⟩).1
+                    simp only [OBdd.low_heap_eq_heap] at this
+                    absurd this
+                    apply OBdd.not_oedge_reachable
+                    exact oedge_of_low
+              )
+          ⟨ r,
+            invv,
+            (by rw [O_root_def, U_root_def] at hv; exact hv),
+            .trans hsl (.trans hsh hsv),
+            by
+              constructor
+              swap
+              · rw [← O_root_def, ← U_root_def]
+                exact hvp.2
+              intro k
+              constructor
+              · intro p hp
+                apply (hvp.1 _).1
+                apply (hhp.1 _).1
+                apply (hlp.1 _).1
+                exact hp
+              · constructor
+                · intro hk
+                  apply (hlp.1 _).2.1
+                  apply (hhp.1 _).2.1
+                  apply (hvp.1 _).2.1
+                  exact hk
+                · intro hk hkp
+                  rw [← O_root_def, ← U_root_def]
+                  cases heq : sh.cache[k]? with
+                  | none =>
+                    apply (hvp.1 _).2.2 heq hkp
+                  | some w =>
+                    cases heqq : sl.cache[k]? with
+                    | none =>
+                      have := (hhp.1 _).2.2 heqq ⟨_, heq⟩
+                      constructor
+                      · trans (O.high O_root_def).1.root
+                        · apply OBdd.reachable_of_edge
+                          exact oedge_of_high.2
+                        · exact this.1
+                      · exact this.2
+                    | some ww =>
+                      have := (hlp.1 _).2.2 hk ⟨_, heqq⟩
+                      constructor
+                      · trans (O.low O_root_def).1.root
+                        · apply OBdd.reachable_of_edge
+                          exact oedge_of_low.2
+                        · exact this.1
+                      · exact this.2
+          ⟩
         else
-          if O.1.heap[j].var > U.1.heap[j'].var
+          if hgeq : O.1.heap[j].var.1 > U.1.heap[j'].var.1
           then
-            let l ← apply_helper op O (U.low  U_root_def)
-            let h ← apply_helper op O (U.high U_root_def)
-            heap_push O.1.root U.1.root ⟨U.1.heap[j'].var, l, h⟩
+            let ⟨⟨sl, rl⟩, ⟨invl, hl, hsl, hlp⟩⟩ := apply_helper op O (U.low U_root_def) s0 inv
+            let ⟨⟨sh, rh⟩, ⟨invh, hh, hsh, hhp⟩⟩ := apply_helper op O (U.high U_root_def) sl invl
+            let ⟨r, ⟨invv, hv, hsv, hvp⟩⟩ :=
+              heap_push (O := O) (U := U)
+                ⟨⟨U.1.heap[j'].var.1, by omega⟩, rl, rh⟩ sh invh
+                ⟨_, (hhp.1 _).1 _ hl⟩
+                ⟨_, hh⟩
+                (by
+                  simp only
+                  rw [O_root_def, U_root_def]
+                  simp only [Fin.getElem_fin, toVar_or, le_sup_iff, Fin.is_le', or_true, true_or,
+                    inf_of_le_right, inf_of_le_left]
+                  exact Eq.symm (min_eq_right_of_lt hgeq)
+                )
+                (by
+                  intro j'' hj1
+                  simp only [Fin.getElem_fin]
+                  intro hj2
+                  have := (hhp.1 _).1 _ hl
+                  simp only at this
+                  rw [hj2] at this
+                  have that := (invh.2 _ _ this).1 _ hj1 rfl
+                  simp only at that
+                  rw [that]
+                  exact aux_lt4_low O_root_def U_root_def hgeq
+                )
+                (by
+                  intro j'' hj1
+                  simp only [Fin.getElem_fin]
+                  intro hj2
+                  have := hhp.2 _ hj1 hj2
+                  rw [this]
+                  exact aux_lt4_high O_root_def U_root_def hgeq
+                )
+                (by
+                  intro h0 h1 I
+                  symm
+                  rw [OBdd.evaluate_node'' U_root_def]
+                  simp only
+                  rw [op_if1 op]
+                  simp only [OBdd.evaluate_node]
+                  congr 1
+                  · simp only [Nat.sub_zero, Fin.getElem_fin, Vector.getElem_cast, cook_heap,
+                      RawNode.cook, Vector.getElem_ofFn, Vector.getElem_push_eq, eq_iff_iff,
+                      Bool.coe_iff_coe]
+                    have := Vector.getElem_extract (as := I) (start := 0) (stop := n') (i := U.1.heap[j'.1].var.1) (by omega)
+                    simp only [Nat.sub_zero, zero_add] at this
+                    exact this
+                  · conv =>
+                      rhs
+                      congr
+                      congr
+                      congr
+                      rfl
+                      simp [cook_heap, RawNode.cook]
+                      rfl
+                      rfl
+                    symm
+                    have := (invh.2 ⟨O.1.root, (U.high U_root_def).1.root⟩ rh hh).2
+                    calc _
+                      _ = OBdd.evaluate ⟨⟨cook_heap sh.heap _, rh.cook _⟩, _⟩ I := by
+                        rw [push_evaluate]
+                        · exact this.2.2.1
+                        · exact push_ordered this.2.2.2.1
+                        · exact this.2.2.2.1
+                      _ = _ := by
+                        have := this.2.2.2.2 I
+                        simp only [Vector.take_eq_extract, OBdd.high_heap_eq_heap] at this
+                        exact this
+                  · conv =>
+                      rhs
+                      congr
+                      congr
+                      congr
+                      rfl
+                      simp [cook_heap, RawNode.cook]
+                      rfl
+                      rfl
+                    symm
+                    have : sh.cache[(⟨O.1.root, (U.low U_root_def).1.root⟩ : Pointer m × Pointer m')]? = some rl := by
+                      apply (hhp.1 _).1
+                      exact hl
+                    have := invh.2 ⟨O.1.root, (U.low U_root_def).1.root⟩ rl this
+                    calc _
+                      _ = OBdd.evaluate ⟨⟨cook_heap sh.heap _, rl.cook _⟩, _⟩ I := by
+                        rw [push_evaluate]
+                        · exact this.2.2.2.1
+                        · exact push_ordered this.2.2.2.2.1
+                        · exact this.2.2.2.2.1
+                      _ = _ := by
+                        have := this.2.2.2.2.2 I
+                        simp only [Vector.take_eq_extract, OBdd.high_heap_eq_heap] at this
+                        exact this
+                )
+                (by
+                  simp only [cache_get] at hc
+                  cases heq : sh.cache[(⟨O.1.root, U.1.root⟩ : Pointer m × Pointer m')]? with
+                  | none => rfl
+                  | some val =>
+                    cases heqq : sl.cache[(⟨O.1.root, U.1.root⟩ : Pointer m × Pointer m')]? with
+                    | none =>
+                      have := ((hhp.1 _).2.2 heqq ⟨val, heq⟩).2
+                      simp only [OBdd.high_heap_eq_heap] at this
+                      absurd this
+                      apply OBdd.not_oedge_reachable
+                      exact oedge_of_high
+                    | some val =>
+                      have := ((hlp.1 _).2.2 hc ⟨_, heqq⟩).2
+                      simp only [OBdd.low_heap_eq_heap] at this
+                      absurd this
+                      apply OBdd.not_oedge_reachable
+                      exact oedge_of_low
+                )
+            ⟨ r,
+              invv,
+              (by rw [O_root_def, U_root_def] at hv; exact hv),
+              .trans hsl (.trans hsh hsv),
+              by
+                constructor
+                swap
+                · rw [← O_root_def, ← U_root_def]
+                  exact hvp.2
+                intro k
+                constructor
+                · intro p hp
+                  apply (hvp.1 _).1
+                  apply (hhp.1 _).1
+                  apply (hlp.1 _).1
+                  exact hp
+                · constructor
+                  · intro hk
+                    apply (hlp.1 _).2.1
+                    apply (hhp.1 _).2.1
+                    apply (hvp.1 _).2.1
+                    exact hk
+                  · intro hk hkp
+                    rw [← O_root_def, ← U_root_def]
+                    cases heq : sh.cache[k]? with
+                    | none =>
+                      apply (hvp.1 _).2.2 heq hkp
+                    | some w =>
+                      cases heqq : sl.cache[k]? with
+                      | none =>
+                        have := (hhp.1 _).2.2 heqq ⟨_, heq⟩
+                        constructor
+                        · exact this.1
+                        · trans (U.high U_root_def).1.root
+                          · apply OBdd.reachable_of_edge
+                            exact oedge_of_high.2
+                          · exact this.2
+                      | some ww =>
+                        have := (hlp.1 _).2.2 hk ⟨_, heqq⟩
+                        constructor
+                        · exact this.1
+                        · trans (U.low U_root_def).1.root
+                          · apply OBdd.reachable_of_edge
+                            exact oedge_of_low.2
+                          · exact this.2
+            ⟩
           else
-            let l ← apply_helper op (O.low  O_root_def) (U.low  U_root_def)
-            let h ← apply_helper op (O.high O_root_def) (U.high U_root_def)
-            heap_push O.1.root U.1.root ⟨U.1.heap[j'].var, l, h⟩
+            let ⟨⟨sl, rl⟩, ⟨invl, hl, hsl, hlp⟩⟩ := apply_helper op (O.low O_root_def) (U.low U_root_def) s0 inv
+            let ⟨⟨sh, rh⟩, ⟨invh, hh, hsh, hhp⟩⟩ := apply_helper op (O.high O_root_def) (U.high U_root_def) sl invl
+            let ⟨r, ⟨invv, hv, hsv, hvp⟩⟩ :=
+              heap_push (O := O) (U := U)
+                ⟨⟨U.1.heap[j'].var.1, by omega⟩, rl, rh⟩ sh invh
+                ⟨_, (hhp.1 _).1 _ hl⟩
+                ⟨_, hh⟩
+                (by
+                  simp only
+                  rw [O_root_def, U_root_def]
+                  simp only [Fin.getElem_fin, toVar_or, le_sup_iff, Fin.is_le', or_true, true_or,
+                    inf_of_le_right, inf_of_le_left]
+                  have heeq : O.1.heap[j].var.1 = U.1.heap[j'].var.1 := by omega
+                  simp only [Fin.getElem_fin] at heeq
+                  rw [heeq]
+                  simp only [min_self]
+                )
+                (by
+                  intro j'' hj1
+                  simp only [Fin.getElem_fin]
+                  intro hj2
+                  have := (hhp.1 _).1 _ hl
+                  simp only at this
+                  rw [hj2] at this
+                  have that := (invh.2 _ _ this).1 _ hj1 rfl
+                  simp only at that
+                  rw [that]
+                  exact aux_lt5_low O_root_def U_root_def (by omega)
+                )
+                (by
+                  intro j'' hj1
+                  simp only [Fin.getElem_fin]
+                  intro hj2
+                  have := hhp.2 _ hj1 hj2
+                  rw [this]
+                  exact aux_lt5_high O_root_def U_root_def (by omega)
+                )
+                (by
+                  intro h0 h1 I
+                  symm
+                  rw [OBdd.evaluate_node'' U_root_def]
+                  rw [OBdd.evaluate_node'' O_root_def]
+                  simp only
+                  have heeq : O.1.heap[j].var.1 = U.1.heap[j'].var.1 := by omega
+                  have heo := Vector.getElem_extract (as := I) (start := 0) (stop := n) (i := O.1.heap[j.1].var.1) (by omega)
+                  have heu := Vector.getElem_extract (as := I) (start := 0) (stop := n') (i := U.1.heap[j'.1].var.1) (by omega)
+                  have : (Vector.cast (m := n') (by omega) (I.extract 0 n'))[U.1.heap[j'].var] = (Vector.cast (m := n) (by omega) (I.extract 0 n))[O.1.heap[j].var] := by
+                    simp only [Fin.getElem_fin]
+                    rw [Vector.getElem_cast]
+                    rw [Vector.getElem_cast]
+                    rw [heo]
+                    rw [heu]
+                    simp only [zero_add]
+                    congr 1
+                    symm
+                    exact heeq
+                  rw [this]
+                  rw [op_if3 op]
+                  simp only [OBdd.evaluate_node]
+                  congr 1
+                  ·
+                    simp only [Nat.sub_zero, Fin.getElem_fin, Vector.getElem_cast, cook_heap,
+                      RawNode.cook, Vector.getElem_ofFn, Vector.getElem_push_eq, eq_iff_iff,
+                      Bool.coe_iff_coe]
+                    simp only [zero_add] at heo
+                    simp_all only [getElem?_eq_none_iff, OBdd.low_heap_eq_heap, forall_exists_index,
+                      Prod.forall, OBdd.high_heap_eq_heap, Fin.getElem_fin, Nat.sub_zero, zero_add,
+                      Vector.getElem_cast]
+                  ·
+                    conv =>
+                      rhs
+                      congr
+                      congr
+                      congr
+                      rfl
+                      simp [cook_heap, RawNode.cook]
+                      rfl
+                      rfl
+                    symm
+                    have := (invh.2 ⟨(O.high O_root_def).1.root, (U.high U_root_def).1.root⟩ rh hh).2.2
+                    calc _
+                      _ = OBdd.evaluate ⟨⟨cook_heap sh.heap _, rh.cook _⟩, _⟩ I := by
+                        rw [push_evaluate]
+                        · exact this.2.1
+                        · exact push_ordered this.2.2.1
+                        · exact this.2.2.1
+                      _ = _ := by
+                        have := this.2.2.2 I
+                        simp only [Vector.take_eq_extract, OBdd.high_heap_eq_heap] at this
+                        exact this
+                  ·
+                    conv =>
+                      rhs
+                      congr
+                      congr
+                      congr
+                      rfl
+                      simp [cook_heap, RawNode.cook]
+                      rfl
+                      rfl
+                    symm
+                    have : sh.cache[(⟨(O.low O_root_def).1.root, (U.low U_root_def).1.root⟩ : Pointer m × Pointer m')]? = some rl := by
+                      apply (hhp.1 _).1
+                      exact hl
+                    have := invh.2 ⟨(O.low O_root_def).1.root, (U.low U_root_def).1.root⟩ rl this
+                    calc _
+                      _ = OBdd.evaluate ⟨⟨cook_heap sh.heap _, rl.cook _⟩, _⟩ I := by
+                        rw [push_evaluate]
+                        · exact this.2.2.2.1
+                        · exact push_ordered this.2.2.2.2.1
+                        · exact this.2.2.2.2.1
+                      _ = _ := by
+                        have := this.2.2.2.2.2 I
+                        simp only [Vector.take_eq_extract, OBdd.high_heap_eq_heap] at this
+                        exact this
+                )
+                (by
+                  simp only [cache_get] at hc
+                  cases heq : sh.cache[(⟨O.1.root, U.1.root⟩ : Pointer m × Pointer m')]? with
+                  | none => rfl
+                  | some val =>
+                    cases heqq : sl.cache[(⟨O.1.root, U.1.root⟩ : Pointer m × Pointer m')]? with
+                    | none =>
+                      have := ((hhp.1 _).2.2 heqq ⟨val, heq⟩).2
+                      simp only [OBdd.high_heap_eq_heap] at this
+                      absurd this
+                      apply OBdd.not_oedge_reachable
+                      exact oedge_of_high
+                    | some val =>
+                      have := ((hlp.1 _).2.2 hc ⟨_, heqq⟩).2
+                      simp only [OBdd.low_heap_eq_heap] at this
+                      absurd this
+                      apply OBdd.not_oedge_reachable
+                      exact oedge_of_low
+                )
+          ⟨ r,
+            invv,
+            (by rw [O_root_def, U_root_def] at hv; exact hv),
+            .trans hsl (.trans hsh hsv),
+            by
+              constructor
+              swap
+              · rw [← O_root_def, ← U_root_def]
+                exact hvp.2
+              intro k
+              constructor
+              · intro p hp
+                apply (hvp.1 _).1
+                apply (hhp.1 _).1
+                apply (hlp.1 _).1
+                exact hp
+              · constructor
+                · intro hk
+                  apply (hlp.1 _).2.1
+                  apply (hhp.1 _).2.1
+                  apply (hvp.1 _).2.1
+                  exact hk
+                · intro hk hkp
+                  rw [← O_root_def, ← U_root_def]
+                  cases heq : sh.cache[k]? with
+                  | none =>
+                    apply (hvp.1 _).2.2 heq hkp
+                  | some w =>
+                    cases heqq : sl.cache[k]? with
+                    | none =>
+                      have := (hhp.1 _).2.2 heqq ⟨_, heq⟩
+                      constructor
+                      · trans (O.high O_root_def).1.root
+                        · apply OBdd.reachable_of_edge
+                          exact oedge_of_high.2
+                        · exact this.1
+                      · trans (U.high U_root_def).1.root
+                        · apply OBdd.reachable_of_edge
+                          exact oedge_of_high.2
+                        · exact this.2
+                    | some ww =>
+                      have := (hlp.1 _).2.2 hk ⟨_, heqq⟩
+                      constructor
+                      · trans (O.low O_root_def).1.root
+                        · apply OBdd.reachable_of_edge
+                          exact oedge_of_low.2
+                        · exact this.1
+                      · trans (U.low U_root_def).1.root
+                        · apply OBdd.reachable_of_edge
+                          exact oedge_of_low.2
+                        · exact this.2
+          ⟩
 termination_by (O, U)
 decreasing_by
   · right; exact oedge_of_low
@@ -131,165 +1536,24 @@ decreasing_by
   · left;  exact oedge_of_high
   · right; exact oedge_of_low
   · right; exact oedge_of_high
-  · left;  exact oedge_of_low
-  · left;  exact oedge_of_high
+  · left; exact oedge_of_low
+  · left; exact oedge_of_high
 
-def apply {n m m' : Nat} : (Bool → Bool → Bool) → OBdd n.succ m → OBdd n.succ m' → Bdd n.succ (p2t m m') := fun op O U ↦
-  let ⟨root, state⟩ := apply_helper op O U ⟨Std.HashMap.emptyWithCapacity, Vector.replicate _ ⟨0, .terminal false, .terminal false⟩, 0⟩
-  ⟨state.heap, root⟩
-
-def apply' {n n' m m' p : Nat} : max n n' = p.succ → (Bool → Bool → Bool) → OBdd n m → OBdd n' m' → OBdd (max n n') (p2t m m') := fun h op O U ↦
-  ⟨h ▸ apply op (h ▸ Lift.olift (n' := max n n') (Nat.le_max_left ..) O) (h ▸ Lift.olift (n' := max n n') (Nat.le_max_right ..) U), sorry⟩
-
-
--- theorem apply_helper_spec' {n m m' : Nat} {op : (Bool → Bool → Bool)} {O : OBdd n m} {U : OBdd n m'} {s : State n m m'} :
---     GoodState op O.1.heap U.1.heap s →
---     let ⟨root, s'⟩ := apply_helper op O U s
---     ∃ (o : Bdd.Ordered ⟨s'.heap, root⟩), ∀ I, (op (O.evaluate I) (U.evaluate I)) = OBdd.evaluate ⟨⟨s'.heap, root⟩, o⟩ I := by
---   intro sg
---   split
---   next final_root final_state h =>
---     unfold apply_helper at h
---     simp only [bind, StateT.bind] at h
---     split at h
---     next hit s' heq =>
---       cases hit with
---       | some val =>
---         simp only [pure, StateT.pure] at h
---         rw [Prod.mk.injEq] at h
---         have := sg ⟨O.1.root, U.1.root⟩ (mem_cache_of_cache_get_eq_some (Option.isSome_iff_exists.mpr ⟨val, (by rw [heq])⟩))
---         simp only at this
---         rw [show { heap := O.1.heap, root := O.1.root } = O.1 by rfl] at this
---         sorry
---       | none =>
---         sorry
-
-private theorem apply_helper_spec {n m m' : Nat} {op : (Bool → Bool → Bool)} {O : OBdd n m} {U : OBdd n m'} {initial_state : State n m m'} :
-    GoodState op O.1.heap U.1.heap initial_state →
-    let ⟨root, s'⟩ := apply_helper op O U initial_state
-    GoodState op O.1.heap U.1.heap s' ∧
-    ∃ (o : Bdd.Ordered ⟨s'.heap, root⟩), ∀ I, (op (O.evaluate I) (U.evaluate I)) = OBdd.evaluate ⟨⟨s'.heap, root⟩, o⟩ I := by
-  intro sg
-  split
-  next final_root final_state h =>
-    unfold apply_helper at h
-    split at h
-    next b heq =>
-      split at h
-      next b' heqq =>
-        simp only [bind, StateT.bind] at h
-        split at h
-        next a s'' heqqq =>
-          split at h
-          next root =>
-            -- cache hit!
-            simp only [pure, StateT.pure] at h
-            rw [Prod.mk.injEq] at h
-            have := (mem_cache_of_cache_get_eq_some (Option.isSome_iff_exists.mpr ⟨root, (by rw [heqqq])⟩))
-            rcases (sg ⟨O.1.root, U.1.root⟩ this) with ⟨h1, h2, h3, h4⟩
-            have that : initial_state.cache[(O.1.root, U.1.root)]'this = root := by
-              simp [cache_get] at heqqq
-              rw [Prod.mk.injEq] at heqqq
-              rw [Std.HashMap.getElem?_eq_some_getElem (h' := this)] at heqqq
-              rcases heqqq with ⟨hh1, hh2⟩
-              injection hh1 with hhh1
-            rw [that] at h1
-            rw [← h.1, ← h.2]
-            have : s'' = (cache_get O.1.root U.1.root initial_state).2 := by rw [heqqq]
-            rw [cache_get_preserves_state] at this
-            rw [this]
-            constructor
-            · assumption
-            · use h1
-              intro I
-              have := h4 I
-              convert this
-              exact symm that
-          next =>
-            -- cache miss...
-            simp only [StateT.bind, cache_put, Bdd.Ordered.eq_1, pure, StateT.pure, Id.bind_eq] at h
-            rw [Prod.mk.injEq] at h
-            rw [← h.1, ← h.2]
-            simp only
-            have : s'' = (cache_get O.1.root U.1.root initial_state).2 := by rw [heqqq]
-            rw [cache_get_preserves_state] at this
-            rw [this]
-            rw [this] at h heqqq
-            constructor
-            · simp only [GoodState]
-              intro key hk
-              rw [Std.HashMap.getElem_insert]
-              split
-              next hh =>
-                simp at hh
-                use Bdd.Ordered_of_terminal
-                simp_rw [← hh]
-                use O.2
-                use U.2
-                have : ⟨{ heap := O.1.heap, root := O.1.root }, O.2⟩ = O := rfl
-                simp_rw [this]
-                have : ⟨{ heap := U.1.heap, root := U.1.root }, U.2⟩ = U := rfl
-                simp_rw [this]
-                intro I
-                rw [OBdd.evaluate_terminal' heq, OBdd.evaluate_terminal' heqq]
-                simp
-              next hh =>
-                have : key ∈ initial_state.cache := by
-                  apply Std.HashMap.mem_of_mem_insert hk
-                  simp_all only [beq_eq_false_iff_ne]
-                exact sg key this
-            · use Bdd.Ordered_of_terminal
-              intro I
-              rw [OBdd.evaluate_terminal' heq, OBdd.evaluate_terminal' heqq]
-              simp
-      next j' heqq =>
-        simp only [bind, StateT.bind] at h
-        split at h
-        next a s heqqq =>
-          split at h
-          next root => sorry --cache hit
-          next =>
-            simp only [StateT.bind, Id.bind_eq, pure, StateT.pure] at h
---            generalize hh : (apply_helper op O (U.low heqq) s) = sss at h
-            rcases hh : (apply_helper op O (U.low heqq) s) with ⟨ll, s'⟩
-            rcases hhh : (apply_helper op O (U.high heqq) s') with ⟨hl, s''⟩
-            rw [hh, hhh] at h
-            simp only [next] at h
-            have : s = (cache_get O.1.root U.1.root initial_state).2 := by rw [heqqq]
-            rw [cache_get_preserves_state] at this
-            rw [this] at hh
-            have : GoodState op O.1.heap U.1.heap (apply_helper op O (U.low heqq) initial_state).2 := (apply_helper_spec (by rw [OBdd.low_heap_eq_heap]; assumption)).1
-            rw [show (apply_helper op O (U.low heqq) initial_state).2 = s' by rw [hh]] at this
-            have : GoodState op O.1.heap U.1.heap (apply_helper op O (U.high heqq) s').2 := (apply_helper_spec (by rw [OBdd.high_heap_eq_heap]; assumption)).1
-            rw [show (apply_helper op O (U.high heqq) s').2 = s'' by rw [hhh]] at this
-            constructor
-            · rw [← show (heap_push O.1.root U.1.root { var := U.1.heap[j'].var, low := ll, high := hl } s'').2 = final_state by rw [h]]
-              intro key
-              simp only [heap_push]
-              intro hk
-
-              simp only [GoodState, Bdd.Ordered.eq_1, Bdd.Ordered, Prod.forall]
-              sorry
-            · sorry
-    next j heq =>
-      split at h
-      next => sorry
-      next =>
-        split at h
-        sorry
-        sorry
-termination_by (O, U)
-decreasing_by
-  · right; exact oedge_of_low
-  · right; exact oedge_of_high
-
-
-theorem apply_spec {n m m' : Nat} {op : (Bool → Bool → Bool)} {O : OBdd n.succ m} {U : OBdd n.succ m'} :
-    ∃ (o : Bdd.Ordered (apply op O U)), ∀ I, (op (O.evaluate I) (U.evaluate I)) = OBdd.evaluate ⟨apply op O U, o⟩ I :=
-  (apply_helper_spec (by sorry)).2
-
-theorem apply'_spec {n n' m m' p : Nat} {h : max n n' = p.succ} {op : Bool → Bool → Bool} {O : OBdd n m} {U : OBdd n' m'} :
-    ∀ I : Vector Bool (n ⊔ n'), (op ((Lift.olift (by simp) O).evaluate I) ((Lift.olift (by simp) U).evaluate I)) = OBdd.evaluate (apply' h op O U) I := by
-  sorry
+def oapply (op : Bool → Bool → Bool) (O : OBdd n m) (U : OBdd n' m') :
+    (s : Nat) ×
+    { OU : OBdd (n ⊔ n') s //
+      ∀ I,
+        OBdd.evaluate OU I =
+        (op
+          (OBdd.evaluate O (Vector.cast (by simp) (I.take n)))
+          (OBdd.evaluate U (Vector.cast (by simp) (I.take n'))))
+    } :=
+  let ⟨⟨state, root⟩, inv, ps⟩ := apply_helper op O U initial inv_initial
+  ⟨ state.size,
+    ⟨⟨cook_heap state.heap inv.1,
+    root.cook (inv.2 _ root ps.1).2.2.2.1⟩,
+    (inv.2 _ root ps.1).2.2.2.2.1⟩,
+    (inv.2 _ root ps.1).2.2.2.2.2
+  ⟩
 
 end Apply
