SatSolver.lean
@@ -1,0 +1,33 @@
+import Bdd.Sat
+import Std.Sat.CNF.Basic
+
+def parseDimacs (n : Nat) [NeZero n] (lines : List String) : Std.Sat.CNF (Fin n) :=
+  lines.filter (fun l => ¬l.startsWith "p" ∧ ¬l.startsWith "c")
+       |>.map (fun l =>
+         l.trim.splitOn " "
+         |>.filterMap (fun s =>
+           match s.toInt? with
+           | some 0 => none
+           | some i => some (if i > 0 then ⟨i.natAbs, true⟩ else ⟨i.natAbs, false⟩)
+           | none   => none)
+       )
+
+partial def readLines (s : IO.FS.Stream) : IO (List String) := do
+  let line ← s.getLine
+  if line == "" then pure []
+  else let rest ← readLines s; pure (line :: rest)
+
+def main (args : List String) : IO Unit := do
+  match args with
+  | [ns, fs] =>
+    try
+      let handle ← (IO.FS.Handle.mk fs .read)
+      let stream := IO.FS.Stream.ofHandle handle
+      let lines ← readLines stream
+      let cnf := parseDimacs (ns.toNat! + 1) lines
+      if Std.Sat.CNF.Unsat cnf
+      then IO.println "UNSAT"
+      else IO.println "SAT"
+    catch e =>
+      IO.println s!"Error reading file {fs}: {e}"
+  | _ => IO.println "Usage: sat <n> <filename>"
